theories/SOL/Util/Tarski.v
@@ -18,8 +18,28 @@ Arguments get_indi {_} _ _.
 Arguments get_func {_} _ _.
 Arguments get_pred {_} _ _.
 
-
 Notation "⟨ a , b , c ⟩" := (new_env a b c).
+
+(** Type class for ⊨ notations *)
+Class Ent X Y `{funcs_signature, preds_signature} := ent : X -> Y -> Prop.
+Notation "X ⊨ phi" := (ent X phi) (at level 20).
+Class Ent' X `{funcs_signature, preds_signature} := ent' : forall M : Model, env (M_domain M) -> X -> Prop.
+Notation "( M , rho ) ⊨ phi" := (ent' M rho phi) (at level 0).
+
+#[global] Instance ent_env `{funcs_signature, preds_signature} domain I : Ent (env domain) form := 
+  @sat _ _ domain I.
+#[global] Instance ent'_form `{funcs_signature, preds_signature} : Ent' form :=
+  fun M rho phi => @sat _ _ (M_domain M) (M_interp M) rho phi.
+#[global] Instance ent_model `{funcs_signature, preds_signature} : Ent Model form := 
+  fun M phi => forall rho, @sat _ _ (M_domain M) (M_interp M) rho phi.
+#[global] Instance ent_model_theory `{funcs_signature, preds_signature} : Ent Model (form -> Prop) := 
+  fun M T => forall phi, T phi -> M ⊨ phi.
+#[global] Instance ent_theory `{funcs_signature, preds_signature} : Ent (form -> Prop) form := 
+  fun T phi => forall (M : Model) rho, (forall psi, T psi -> (M, rho) ⊨ psi) -> (M, rho) ⊨ phi.
+#[global] Instance ent'_theory `{funcs_signature, preds_signature} : Ent' (form -> Prop) :=
+  fun M rho T => forall phi, T phi -> (M, rho) ⊨ phi.
+#[global] Instance ent'_form' `{funcs_signature, preds_signature} : Ent' form :=
+  fun M rho phi => @sat _ _ (M_domain M) (M_interp M) rho phi.
 
 
 Section Environment.
